Cleanup and moving some stuff to public repo

hol/p4_exec_semSyntax.sig
@@ -3,7 +3,7 @@ sig
   include Abbrev
 
 val arch_multi_exec_tm : term
-val dest_arch_multi_exec : term -> term * term * term
+val dest_arch_multi_exec : term -> term * term * term * term
 val is_arch_multi_exec : term -> bool
 val mk_arch_multi_exec : term * term * int -> term
 
