hol/retrofit_sem/p4_exec_wrapper_ffiLib.sml
@@ -826,7 +826,7 @@ fun translate_p4 progname actx astate n_max debug_mode inlogic =
      (* TODO: Fix option type? *)
      val cake_top_exec_def =
       Define
-       ‘cake_top_exec input = SOME $ p4_get_output_list (arch_multi_exec_total ^actx (p4_append_input_list [input] ^astate) ^n_max)’;
+       ‘cake_top_exec input = SOME $ p4_get_output_list (arch_multi_exec_total_zero ^actx (p4_append_input_list [input] ^astate) ^n_max)’;
 
      (* TODO: This is the bottleneck... *)
      val _ = translate cake_top_exec_def;
